ContextTypeLanguage/theories/WF.v
@@ -1,8 +1,132 @@
-(** * ContextTypeLanguage.WFContextTy
+(** * ContextTypeLanguage.WF
+
+    Formation/scoping predicates for lvar sets, context types, and contexts. *)
+
+From LocallyNameless Require Import Classes.
+From ContextTypeLanguage Require Export LtyEnv.
+From ContextBase Require Import BaseTactics.
+
+(** * ContextTypeLanguage.WF
+
+    Formation/scoping predicates for logic-variable sets. *)
+
+
+Definition lvar_wf_at (d : nat) (D : aset) (v : logic_var) : Prop :=
+  match v with
+  | LVFree x => x ∈ D
+  | LVBound k => k < d
+  end.
+
+Definition lvars_wf_at (d : nat) (D : aset) (L : lvset) : Prop :=
+  forall v, v ∈ L -> lvar_wf_at d D v.
+
+Definition lvars_lc_at (d : nat) (L : lvset) : Prop :=
+  forall k, k ∈ lvars_bv L -> k < d.
+
+Lemma lvars_wf_at_mono d D E L :
+  D ⊆ E ->
+  lvars_wf_at d D L ->
+  lvars_wf_at d E L.
+Proof.
+  intros HDE Hwf [k|x] Hin; cbn [lvar_wf_at] in *.
+  - exact (Hwf (LVBound k) Hin).
+  - apply HDE. exact (Hwf (LVFree x) Hin).
+Qed.
+
+Lemma lvars_wf_at_lc d D L :
+  lvars_wf_at d D L ->
+  lvars_lc_at d L.
+Proof.
+  intros Hwf k Hk.
+  rewrite lvars_bv_elem in Hk.
+  exact (Hwf (LVBound k) Hk).
+Qed.
+
+Lemma lvars_wf_at_fv_subset d D L :
+  lvars_wf_at d D L ->
+  lvars_fv L ⊆ D.
+Proof.
+  intros Hwf x Hx.
+  apply lvars_fv_elem in Hx.
+  exact (Hwf (LVFree x) Hx).
+Qed.
+
+Lemma lvars_wf_at_drop_fresh d D x L :
+  x ∉ lvars_fv L ->
+  lvars_wf_at d (D ∪ {[x]}) L ->
+  lvars_wf_at d D L.
+Proof.
+  intros Hfresh Hwf [k|y] Hy; cbn [lvar_wf_at].
+  - exact (Hwf (LVBound k) Hy).
+  - assert (y ∈ D ∪ {[x]}) as HyD by exact (Hwf (LVFree y) Hy).
+    apply elem_of_union in HyD as [HyD | Hyx]; [exact HyD |].
+    rewrite elem_of_singleton in Hyx. subst y.
+    exfalso. apply Hfresh. apply lvars_fv_elem. exact Hy.
+Qed.
+
+Lemma lvars_wf_at_open_body D L x :
+  x ∉ D ->
+  lvars_wf_at 1 D L ->
+  lvars_wf_at 0 (D ∪ {[x]}) (lvars_open 0 x L).
+Proof.
+  intros Hx Hwf v Hv.
+  rewrite set_swap_elem in Hv.
+  destruct v as [k|y]; cbn [lvar_wf_at].
+  - destruct k as [|k].
+    + rewrite swap_l in Hv.
+      assert (LVFree x ∈ L) as Hxin by exact Hv.
+      exfalso. apply Hx. exact (Hwf (LVFree x) Hxin).
+    + exfalso.
+      base_swap_normalize.
+      assert (LVBound (S k) ∈ L) as Hk.
+      { exact Hv. }
+      specialize (Hwf (LVBound (S k)) Hk). cbn [lvar_wf_at] in Hwf. lia.
+  - destruct (decide (x = y)) as [->|Hxy].
+    + set_solver.
+    + assert (LVFree y ∈ L) as Hy.
+      { base_swap_normalize. exact Hv. }
+      apply elem_of_union. left. exact (Hwf (LVFree y) Hy).
+Qed.
+
+Lemma lvars_wf_at_open_at d D L x :
+  x ∉ D ->
+  lvars_wf_at (S d) D L ->
+  lvars_wf_at d (D ∪ {[x]}) (lvars_open d x L).
+Proof.
+  intros Hx Hwf v Hv.
+  rewrite set_swap_elem in Hv.
+  destruct v as [k|y]; cbn [lvar_wf_at].
+  - destruct (decide (k = d)) as [->|Hkd].
+    + rewrite swap_l in Hv.
+      exfalso. apply Hx. exact (Hwf (LVFree x) Hv).
+    + base_swap_normalize.
+      specialize (Hwf (LVBound k) Hv). cbn [lvar_wf_at] in Hwf.
+      lia.
+  - destruct (decide (x = y)) as [->|Hxy].
+    + apply elem_of_union_r. set_solver.
+    + base_swap_normalize.
+      apply elem_of_union_l. exact (Hwf (LVFree y) Hv).
+Qed.
+
+Lemma lvars_wf_at_shift d D L k :
+  d <= k ->
+  lvars_wf_at d D L ->
+  lvars_wf_at d D (lvars_shift_from k L).
+Proof.
+  intros Hdk Hwf v Hv.
+  unfold lvars_shift_from in Hv.
+  apply elem_of_map in Hv as [u [-> Hu]].
+  destruct u as [n|x]; cbn [logic_var_shift_from lvar_wf_at].
+  - destruct (decide (k <= n)) as [Hkn|Hkn].
+    + specialize (Hwf (LVBound n) Hu). cbn [lvar_wf_at] in Hwf. lia.
+    + exact (Hwf (LVBound n) Hu).
+  - exact (Hwf (LVFree x) Hu).
+Qed.
+
+(** * ContextTypeLanguage.WF
 
     Formation/scoping predicates for context types. *)
 
-From ContextTypeLanguage Require Export WFLvars.
 
 Fixpoint cty_lc_at (d : nat) (τ : context_ty) : Prop :=
   match τ with
@@ -777,3 +901,332 @@ Proof.
   intros H.
   eapply wf_context_ty_at_shift; [lia|exact H].
 Qed.
+
+(** * ContextTypeLanguage.WF
+
+    Formation/scoping predicates for type contexts. *)
+
+
+Fixpoint basic_ctx (D : aset) (Γ : ctx) : Prop :=
+  match Γ with
+  | CtxEmpty => True
+  | CtxBind x τ =>
+      x ∉ D /\ basic_context_ty D τ
+  | CtxComma Γ1 Γ2 =>
+      basic_ctx D Γ1 /\
+      basic_ctx (D ∪ ctx_dom Γ1) Γ2 /\
+      ctx_dom Γ1 ## ctx_dom Γ2
+  | CtxStar Γ1 Γ2 =>
+      basic_ctx D Γ1 /\
+      basic_ctx D Γ2 /\
+      ctx_dom Γ1 ## ctx_dom Γ2
+  | CtxSum Γ1 Γ2 =>
+      basic_ctx D Γ1 /\
+      basic_ctx D Γ2 /\
+      ctx_dom Γ1 = ctx_dom Γ2 /\
+      erase_ctx Γ1 = erase_ctx Γ2
+  end.
+
+#[global] Instance scoped_ctx : ScopedIn ctx := basic_ctx.
+
+Notation "D '⊢sΓ' Γ" := (basic_ctx D Γ)
+  (at level 40, Γ at level 40, only printing).
+
+Lemma scoped_ctx_iff D Γ :
+  D ⊢s Γ <-> basic_ctx D Γ.
+Proof. reflexivity. Qed.
+
+Lemma basic_ctx_weaken_fresh D E Γ :
+  D ⊆ E ->
+  ctx_dom Γ ## E ->
+  basic_ctx D Γ ->
+  basic_ctx E Γ.
+Proof.
+  induction Γ in D, E |- *; cbn [basic_ctx ctx_dom]; intros HDE Hdom Hbasic.
+  - exact I.
+  - destruct Hbasic as [Hx Hτ]. split.
+    + set_solver.
+    + eapply basic_context_ty_mono; [exact HDE|exact Hτ].
+  - destruct Hbasic as [H1 [H2 Hdisj]]. repeat split.
+    + eapply IHΓ1; [exact HDE|set_solver|exact H1].
+    + eapply (IHΓ2 (D ∪ ctx_dom Γ1) (E ∪ ctx_dom Γ1)).
+      * set_solver.
+      * set_solver.
+      * exact H2.
+    + exact Hdisj.
+  - destruct Hbasic as [H1 [H2 Hdisj]]. repeat split.
+    + eapply IHΓ1; [exact HDE|set_solver|exact H1].
+    + eapply IHΓ2; [exact HDE|set_solver|exact H2].
+    + exact Hdisj.
+  - destruct Hbasic as [H1 [H2 [Hdom12 Herase]]]. repeat split.
+    + eapply IHΓ1; [exact HDE|set_solver|exact H1].
+    + eapply IHΓ2; [exact HDE|set_solver|exact H2].
+    + exact Hdom12.
+    + exact Herase.
+Qed.
+
+Lemma basic_ctx_fv_subset D Γ :
+  basic_ctx D Γ ->
+  ctx_fv Γ ⊆ D.
+Proof.
+  induction Γ in D |- *; cbn [basic_ctx ctx_fv ctx_dom]; intros Hbasic.
+  - set_solver.
+  - destruct Hbasic as [_ Hτ].
+    apply basic_context_ty_fv_subset. exact Hτ.
+  - destruct Hbasic as [H1 [H2 _]].
+    specialize (IHΓ1 D H1).
+    specialize (IHΓ2 (D ∪ ctx_dom Γ1) H2).
+    set_solver.
+  - destruct Hbasic as [H1 [H2 _]].
+    specialize (IHΓ1 D H1).
+    specialize (IHΓ2 D H2).
+    set_solver.
+  - destruct Hbasic as [H1 [H2 [_ _]]].
+    specialize (IHΓ1 D H1).
+    specialize (IHΓ2 D H2).
+    set_solver.
+Qed.
+
+Lemma basic_ctx_fv_subset_weak D Γ :
+  basic_ctx D Γ ->
+  ctx_fv Γ ⊆ D ∪ ctx_dom Γ.
+Proof.
+  intros Hbasic.
+  pose proof (basic_ctx_fv_subset D Γ Hbasic). set_solver.
+Qed.
+
+Lemma basic_ctx_dom_fresh D Γ :
+  basic_ctx D Γ ->
+  ctx_dom Γ ## D.
+Proof.
+  induction Γ in D |- *; cbn [basic_ctx ctx_dom]; intros Hbasic.
+  - set_solver.
+  - destruct Hbasic as [Hx _]. set_solver.
+  - destruct Hbasic as [H1 [H2 Hdisj]].
+    specialize (IHΓ1 D H1).
+    specialize (IHΓ2 (D ∪ ctx_dom Γ1) H2).
+    set_solver.
+  - destruct Hbasic as [H1 [H2 _]].
+    specialize (IHΓ1 D H1).
+    specialize (IHΓ2 D H2).
+    set_solver.
+  - destruct Hbasic as [H1 [H2 [_ _]]].
+    specialize (IHΓ1 D H1).
+    specialize (IHΓ2 D H2).
+    set_solver.
+Qed.
+
+Lemma basic_ctx_dom_fv_disjoint D Γ :
+  basic_ctx D Γ ->
+  ctx_dom Γ ## ctx_fv Γ.
+Proof.
+  intros Hbasic.
+  pose proof (basic_ctx_dom_fresh D Γ Hbasic).
+  pose proof (basic_ctx_fv_subset D Γ Hbasic).
+  set_solver.
+Qed.
+
+Lemma basic_ctx_bind_lc D x τ :
+  basic_ctx D (CtxBind x τ) ->
+  lc_context_ty τ.
+Proof.
+  intros [_ Hτ]. apply (basic_context_ty_lc D). exact Hτ.
+Qed.
+
+Lemma basic_ctx_lc D Γ :
+  basic_ctx D Γ ->
+  forall x τ, Γ = CtxBind x τ -> lc_context_ty τ.
+Proof.
+  intros Hbasic x τ ->.
+  apply (basic_ctx_bind_lc D x τ). exact Hbasic.
+Qed.
+
+Lemma basic_ctx_erase_dom D Γ :
+  basic_ctx D Γ ->
+  dom (erase_ctx Γ) = ctx_dom Γ.
+Proof.
+  induction Γ in D |- *; cbn [basic_ctx erase_ctx ctx_dom]; intros Hbasic.
+  - rewrite dom_empty_L. reflexivity.
+  - apply (dom_singleton_L (M := gmap atom) (D := gset atom)).
+  - destruct Hbasic as [H1 [H2 _]].
+    change (dom (erase_ctx Γ1 ∪ erase_ctx Γ2) = ctx_dom Γ1 ∪ ctx_dom Γ2).
+    transitivity (dom (erase_ctx Γ1) ∪ dom (erase_ctx Γ2)).
+    + apply (dom_union_L (M := gmap atom) (D := gset atom)).
+    + rewrite (IHΓ1 D) by exact H1.
+      rewrite (IHΓ2 (D ∪ ctx_dom Γ1)) by exact H2.
+      reflexivity.
+  - destruct Hbasic as [H1 [H2 _]].
+    change (dom (erase_ctx Γ1 ∪ erase_ctx Γ2) = ctx_dom Γ1 ∪ ctx_dom Γ2).
+    transitivity (dom (erase_ctx Γ1) ∪ dom (erase_ctx Γ2)).
+    + apply (dom_union_L (M := gmap atom) (D := gset atom)).
+    + rewrite (IHΓ1 D) by exact H1.
+      rewrite (IHΓ2 D) by exact H2.
+      reflexivity.
+  - destruct Hbasic as [H1 [_ [Hdom _]]].
+    rewrite (IHΓ1 D) by exact H1.
+    set_solver.
+Qed.
+
+Lemma basic_ctx_empty_fv Γ :
+  basic_ctx ∅ Γ ->
+  ctx_fv Γ ⊆ ctx_dom Γ.
+Proof.
+  intros Hbasic.
+  pose proof (basic_ctx_fv_subset ∅ Γ Hbasic).
+  set_solver.
+Qed.
+
+(** * ContextTypeLanguage.Notation
+
+    Public surface for the type-language layer.  Other layers should import
+    this file instead of reaching into the implementation files directly. *)
+
+
+Definition basic_qualifier (D : aset) (q : type_qualifier) : Prop :=
+  lvars_wf_at 0 D (qual_vars q).
+
+Definition basic_qualifier_body (D : aset) (q : type_qualifier) : Prop :=
+  lvars_wf_at 1 D (qual_vars q).
+
+Lemma basic_qualifier_lc D q :
+  basic_qualifier D q ->
+  lc_qualifier q.
+Proof.
+  intros Hwf [k|x] Hv; cbn [lc_logic_var_key].
+  - exfalso.
+    specialize (Hwf (LVBound k) Hv). cbn [lvar_wf_at] in Hwf. lia.
+  - exact I.
+Qed.
+
+Lemma basic_qualifier_body_lc D q :
+  basic_qualifier_body D q ->
+  body_qualifier q.
+Proof.
+  intros Hwf.
+  exists D. intros x Hx.
+  apply basic_qualifier_lc with (D := D ∪ {[x]}).
+  unfold basic_qualifier.
+  rewrite qual_open_atom_vars.
+  apply lvars_wf_at_open_body; assumption.
+Qed.
+
+Lemma basic_qualifier_fv_subset D q :
+  basic_qualifier D q ->
+  qual_dom q ⊆ D.
+Proof.
+  apply lvars_wf_at_fv_subset.
+Qed.
+
+Lemma basic_qualifier_body_fv_subset D q :
+  basic_qualifier_body D q ->
+  qual_dom q ⊆ D.
+Proof.
+  apply lvars_wf_at_fv_subset.
+Qed.
+
+Lemma basic_qualifier_body_top D :
+  basic_qualifier_body D qual_top.
+Proof.
+  unfold basic_qualifier_body, qual_top. cbn [qual_vars qual_lvars].
+  intros v Hv. set_solver.
+Qed.
+
+Lemma basic_context_ty_over D b q :
+  basic_qualifier_body D q ->
+  basic_context_ty D (CTOver b q).
+Proof.
+  intros Hq.
+  apply basic_context_ty_iff_wf_context_ty_at.
+  exact Hq.
+Qed.
+
+Lemma basic_context_ty_under D b q :
+  basic_qualifier_body D q ->
+  basic_context_ty D (CTUnder b q).
+Proof.
+  intros Hq.
+  apply basic_context_ty_iff_wf_context_ty_at.
+  exact Hq.
+Qed.
+
+Lemma basic_context_ty_inter D τ1 τ2 :
+  basic_context_ty D τ1 ->
+  basic_context_ty D τ2 ->
+  erase_ty τ1 = erase_ty τ2 ->
+  basic_context_ty D (CTInter τ1 τ2).
+Proof.
+  intros H1 H2 Herase.
+  apply basic_context_ty_iff_wf_context_ty_at.
+  cbn [wf_context_ty_at]. repeat split; try assumption;
+    apply basic_context_ty_iff_wf_context_ty_at; assumption.
+Qed.
+
+Lemma basic_ctx_empty D :
+  basic_ctx D CtxEmpty.
+Proof.
+  exact I.
+Qed.
+
+Lemma basic_ctx_bind D x τ :
+  x ∉ D ->
+  basic_context_ty D τ ->
+  basic_ctx D (CtxBind x τ).
+Proof.
+  intros Hx Hτ. split; assumption.
+Qed.
+
+Lemma basic_ctx_star D Γ1 Γ2 :
+  basic_ctx D Γ1 ->
+  basic_ctx D Γ2 ->
+  ctx_dom Γ1 ## ctx_dom Γ2 ->
+  basic_ctx D (CtxStar Γ1 Γ2).
+Proof.
+  intros H1 H2 Hdisj. repeat split; assumption.
+Qed.
+
+Lemma basic_ctx_sum D Γ1 Γ2 :
+  basic_ctx D Γ1 ->
+  basic_ctx D Γ2 ->
+  ctx_dom Γ1 = ctx_dom Γ2 ->
+  erase_ctx Γ1 = erase_ctx Γ2 ->
+  basic_ctx D (CtxSum Γ1 Γ2).
+Proof.
+  intros H1 H2 Hdom Herase. repeat split; assumption.
+Qed.
+
+#[global] Instance OpenFv_qualifier : OpenFv atom type_qualifier.
+Proof.
+  intros q x k.
+  cbn [Stale_atom stale_qualifier].
+  intros y Hy.
+  pose proof (qual_open_atom_dom_subset k x q y Hy) as Hy'.
+  apply elem_of_union in Hy' as [Hyq|Hyx].
+  - apply elem_of_union_r. exact Hyq.
+  - apply elem_of_union_l. exact Hyx.
+Qed.
+
+#[global] Instance OpenFv_cty : OpenFv atom context_ty.
+Proof.
+  intros τ x k.
+  cbn [Stale_atom stale_cty_inst].
+  intros y Hy.
+  pose proof (cty_open_fv_subset k x τ y Hy) as Hy'.
+  apply elem_of_union in Hy' as [Hyτ|Hyx].
+  - apply elem_of_union_r. exact Hyτ.
+  - apply elem_of_union_l. exact Hyx.
+Qed.
+
+#[global] Hint Resolve
+  basic_context_ty_lc
+  basic_context_ty_fv_subset
+  basic_qualifier_lc
+  basic_qualifier_body_lc
+  basic_qualifier_fv_subset
+  basic_qualifier_body_fv_subset
+  basic_ctx_dom_fresh
+  basic_ctx_empty
+  basic_ctx_bind
+  basic_ctx_star
+  basic_ctx_sum
+  : type_lang.
+
